templates/lockfree/skiplist_search.v
@@ -1,0 +1,52 @@
+(* Herlihy Skiplist with a single level : Search *)
+
+From iris.algebra Require Import excl auth cmra gmap agree gset numbers.
+From iris.algebra.lib Require Import dfrac_agree.
+From iris.heap_lang Require Export notation locations lang.
+From iris.base_logic.lib Require Export invariants.
+From iris.program_logic Require Export atomic.
+From iris.proofmode Require Import tactics.
+From iris.heap_lang Require Import proofmode par.
+From iris.heap_lang.lib Require Import nondet_bool.
+From iris.bi.lib Require Import fractional.
+Set Default Proof Using "All".
+From iris.bi.lib Require Import fractional.
+Require Export skiplist_traverse.
+
+  Lemma searchOp_spec (Σ : gFunctors) (H' : heapGS Σ) (H'' : dsG Σ) (H''' : hsG Σ)
+    N γ_t γ_r γ_m γ_mt γ_msy r (p: proph_id) pvs tid t0 Q k (hd tl: Node) :
+      main_inv Σ H' H'' H''' N γ_t γ_r γ_m γ_mt γ_msy r -∗
+      thread_start Σ H' H'' H''' γ_t γ_mt tid t0 -∗
+      □ update_helping_protocol Σ H' H'' H''' N γ_t γ_r γ_mt γ_msy -∗
+      ⌜local_pre (searchOp k)⌝ -∗
+        {{{ proph p pvs ∗ 
+            (match process_proph tid pvs with
+              contra => au Σ H' H'' H''' N γ_r (searchOp k) Q
+            | no_upd => True
+            | upd => au Σ H' H'' H''' N γ_r (searchOp k) Q end) }}}
+              search #hd #tl #k @ ⊤
+        {{{ (res: resT) prf pvs', RET #res;
+            proph p pvs' ∗ ⌜pvs = prf ++ pvs'⌝ ∗
+            (match process_proph tid pvs with
+              contra => ⌜Forall (λ x, x.2 ≠ #tid) prf⌝
+            | no_upd => past_lin_witness Σ H' H'' H''' γ_m (searchOp k) res t0
+            | upd => Q #res ∨ 
+                ⌜Forall (λ x, ¬ is_snd true x ∧ x.2 ≠ #tid) prf⌝ end) }}}.
+  Proof. 
+    iIntros "#HInv #Thd_st #Upd [%HL %Range_k]". 
+    iIntros (Φ) "!# (Hproph & Hmatch) Hpost".
+    wp_lam. wp_pures. 
+    wp_apply (traverse_spec Σ H' H'' H'''); try done.
+    iIntros (preds succs ps ss res) "(Hpreds & Hsuccs & %Len_ps 
+      & %Len_ss & %HpsL & %HssL & #Htr)".  
+    wp_pures. 
+    iAssert (past_lin_witness _ _ _ _ γ_m (searchOp k) res t0)%I as "#PastW".
+    { iDestruct "Htr" as "(_ & Htr)". destruct res.
+      all: iDestruct "Htr" as (s)"(#Past_s & %Hk_s & _)".
+      all: iExists s; iFrame "#"; iPureIntro. all: set_solver. }
+    destruct (process_proph tid pvs) eqn: Hpvs.
+    - iApply ("Hpost" $! res [] pvs). iFrame "Hproph". by iPureIntro.
+    - iApply ("Hpost" $! res [] pvs). iFrame "Hproph". iSplitR. by iPureIntro.
+      iRight. by iPureIntro.
+    - iApply ("Hpost" $! res [] pvs). iFrame "Hproph #". done.
+  Qed.
