templates/lockfree/skiplist_spec.v
@@ -1,0 +1,56 @@
+(* Herlihy Skiplist with a single level : Search *)
+
+From iris.algebra Require Import excl auth cmra gmap agree gset numbers.
+From iris.algebra.lib Require Import dfrac_agree.
+From iris.heap_lang Require Export notation locations lang.
+From iris.base_logic.lib Require Export invariants.
+From iris.program_logic Require Export atomic.
+From iris.proofmode Require Import tactics.
+From iris.heap_lang Require Import proofmode par.
+From iris.heap_lang.lib Require Import nondet_bool.
+From iris.bi.lib Require Import fractional.
+Set Default Proof Using "All".
+From iris.bi.lib Require Import fractional.
+Require Export skiplist_search skiplist_delete skiplist_insert hindsight_proof.
+
+Module SKIPLIST_SPEC : HINDSIGHT_SPEC.
+  Module DS := skiplist_util.SK.
+  Module DEFS := skiplist_util.DEFS.
+  Export DS DEFS.
+  
+  Lemma dsOp_spec (Σ : gFunctors) (H' : heapGS Σ) (H'' : dsG Σ) (H''' : hsG Σ)
+    N γ_t γ_r γ_m γ_mt γ_msy r op (p: proph_id) pvs tid t0 Q :
+          main_inv Σ H' H'' H''' N γ_t γ_r γ_m γ_mt γ_msy r -∗
+          thread_start Σ H' H'' H''' γ_t γ_mt tid t0 -∗
+          □ update_helping_protocol Σ H' H'' H''' N γ_t γ_r γ_mt γ_msy -∗
+          ⌜local_pre op⌝ -∗
+            {{{ proph p pvs ∗ 
+                (match process_proph tid pvs with
+                  contra => au Σ H' H'' H''' N γ_r op Q
+                | no_upd => True
+                | upd => au Σ H' H'' H''' N γ_r op Q end) }}}
+                  dsOp (Op_to_val op) #p #r @ ⊤
+            {{{ (res: resT) prf pvs', RET #res;
+                proph p pvs' ∗ ⌜pvs = prf ++ pvs'⌝ ∗
+                (match process_proph tid pvs with
+                  contra => ⌜Forall (λ x, x.2 ≠ #tid) prf⌝
+                | no_upd => past_lin_witness Σ H' H'' H''' γ_m op res t0
+                | upd => Q #res ∨ 
+                    ⌜Forall (λ x, ¬ is_snd true x ∧ x.2 ≠ #tid) prf⌝ end) }}}.
+  Proof.
+    iIntros "#HInv #Thd #HUpd %Local". unfold dsOp. 
+    iIntros (Φ) "!# Hpre Hpost". 
+    wp_lam. wp_pures. wp_bind (! _)%E.
+    iInv "HInv" as (M0 T0 s0) "(>Ds & >%Habs0 & >Hist & Help & >Templ)".
+    iDestruct "Templ" as (hd tl)"(#HR & SShot0 & Res & %PT0 & %Trans_M0)".
+    wp_load. iModIntro. iSplitR "Hpre Hpost".
+    { iExists M0, T0, s0. iNext. iFrame "%#∗". iExists hd, tl. iFrame "%#". }
+    wp_pures. unfold Op_to_val; destruct op as [k|k|k]; wp_pures.
+    - wp_apply (searchOp_spec with "[] [] [] [] [Hpre]"); try done.
+    - wp_apply (insertOp_spec with "[] [] [] [] [Hpre]"); try done.
+    - wp_apply (deleteOp_spec with "[] [] [] [] [Hpre]"); try done.
+  Qed.
+
+End SKIPLIST_SPEC.
+
+
