templates/util/array_util.v
@@ -1,0 +1,37 @@
+From iris.proofmode Require Import tactics.
+From iris.heap_lang Require Export notation locations lang.
+From iris.heap_lang Require Import proofmode.
+Set Default Proof Using "All".
+From flows Require Export flows.
+
+Definition is_array Σ (Hg1 : heapGS Σ) (array : loc) (xs : list Node) : iProp Σ :=
+  let vs := (fun n => # (LitLoc n)) <$> xs
+  in array ↦∗ vs.
+
+Lemma array_store Σ Hg1 E (i : nat) (v : Node) arr (xs : list Node) :
+  {{{ ⌜i < length xs⌝ ∗ ▷ is_array Σ Hg1 arr xs }}}
+    #(arr +ₗ i) <- #v @ E 
+  {{{ RET #(); is_array Σ Hg1 arr (<[i:=v]>xs) }}}.
+Proof.
+  iIntros (ϕ) "[% isArr] Post".
+  unfold is_array.
+  iApply (wp_store_offset with "isArr").
+  { apply lookup_lt_is_Some_2. by rewrite fmap_length. }
+  rewrite (list_fmap_insert ((λ b : loc, #b) : loc → heap_lang.val) xs i v).
+  iAssumption.
+Qed.
+
+Lemma array_repeat Σ Hg1 (b : Node) (n : nat) :
+  {{{ ⌜0 < n⌝ }}} AllocN #n #b 
+  {{{ arr, RET #arr; is_array Σ Hg1 arr (replicate n b) }}}.
+Proof.
+  iIntros (ϕ ?%inj_lt) "Post".
+  iApply wp_allocN; try done.
+  iNext. iIntros (l) "[lPts _]".
+  iApply "Post".
+  unfold is_array.
+  rewrite Nat2Z.id.
+  rewrite -> fmap_replicate.
+  iAssumption.
+Qed.
+
